concurrency/cancelable_invariants.v
@@ -1,9 +1,11 @@
 (* recapitulate iris/base_logic/lib/cancelable_invariants.v *)
+Require Import Ensembles.
 Require Import VST.msl.shares.
 Require Import VST.veric.shares.
 Require Import VST.msl.ghost.
 Require Import VST.msl.ghost_seplog.
 Require Import VST.veric.invariants.
+Require Import VST.veric.fupd.
 Require Import VST.concurrency.conclib.
 
 #[export] Program Instance share_ghost : Ghost := { G := share; valid _ := True }.
@@ -12,144 +14,83 @@ Definition cinv_own g sh := own(RA := share_ghost) g sh compcert_rmaps.RML.R.Non
 
 Definition cinvariant i g P := invariant i (P || cinv_own g Tsh).
 
-Lemma cinv_alloc' : forall P, wsat * |> P |-- |==> wsat * EX i : _, EX g : _, cinvariant i g P * cinv_own g Tsh.
+Lemma cinvariant_dup : forall i g P, cinvariant i g P = cinvariant i g P * cinvariant i g P.
+Proof.
+  intros; apply invariant_dup.
+Qed.
+
+Lemma cinv_alloc : forall E P, |> P |-- |={E}=> EX i : _, EX g : _, cinvariant i g P * cinv_own g Tsh.
 Proof.
   intros.
   rewrite <- emp_sepcon at 1.
-  eapply derives_trans; [eapply derives_trans, bupd_frame_r|].
-  { apply sepcon_derives, derives_refl.
-    apply (own_alloc(RA := share_ghost)), I. }
-  eapply derives_trans, bupd_trans; apply bupd_mono.
+  sep_eapply (own_alloc(RA := share_ghost)).
+  sep_apply bupd_frame_r.
+  eapply derives_trans, fupd_trans.
+  eapply derives_trans, bupd_fupd; apply bupd_mono.
   Intros g.
-  eapply derives_trans; [eapply derives_trans; [|apply sepcon_derives, derives_refl; unseal_derives; apply wsat_alloc]|].
-  2: { unseal_derives; eapply predicates_hered.derives_trans, own.bupd_mono; [apply own.bupd_frame_r|].
-       rewrite exp_sepcon2, predicates_sl.exp_sepcon2.
-       rewrite predicates_sl.exp_sepcon1.
-       apply predicates_hered.exp_derives; intros.
-       rewrite predicates_sl.sepcon_assoc.
-       apply predicates_sl.sepcon_derives; [apply predicates_hered.derives_refl|].
-       eapply predicates_hered.exp_right, predicates_hered.derives_refl. }
-  rewrite sepcon_comm; apply sepcon_derives, derives_refl.
-  change predicates_sl.sepcon with sepcon; apply sepcon_derives; [apply derives_refl|].
-  change (predicates_hered.box predicates_hered.laterM) with later; apply later_derives, orp_right1, derives_refl.
+  eapply derives_trans; [eapply sepcon_derives, derives_trans, inv_alloc; [apply derives_refl|]|].
+  2: { sep_eapply fupd_frame_l; apply fupd_mono.
+       Intros i; Exists i g.
+       rewrite sepcon_comm; apply derives_refl. }
+  apply later_derives, orp_right1, derives_refl.
 Qed.
 
-Corollary cinv_alloc : forall E P, |> P |-- |={E}=> EX i : _, EX g : _, cinvariant i g P * cinv_own g Tsh.
+Lemma cinv_cancel : forall E i g P, Ensembles.In E i -> cinvariant i g P * cinv_own g Tsh |-- |={E}=> |> P.
 Proof.
   intros.
-  apply wsat_fupd, cinv_alloc'.
+  unfold cinvariant.
+  sep_apply (inv_open E).
+  sep_apply fupd_frame_r; apply fupd_elim.
+  rewrite later_orp, !distrib_orp_sepcon; apply orp_left.
+  - sep_apply (modus_ponens_wand' (cinv_own g Tsh)).
+    { apply orp_right2, now_later. }
+    sep_apply fupd_frame_r; rewrite emp_sepcon; auto.
+  - eapply derives_trans, except_0_fupd.
+    apply orp_right1.
+    rewrite sepcon_assoc; eapply derives_trans; [apply sepcon_derives, now_later; apply derives_refl|].
+    rewrite <- later_sepcon; apply later_derives.
+    rewrite (sepcon_comm _ (cinv_own g Tsh)), <- sepcon_assoc.
+    rewrite sepcon_comm; apply sepcon_FF_derives'.
+    unfold cinv_own; sep_apply own_valid_2; Intros.
+    destruct H0 as (? & J & ?).
+    apply join_Tsh in J as []; contradiction Share.nontrivial.
 Qed.
 
-Lemma cinv_cancel' : forall E i g P, cinvariant i g P * cinv_own g Tsh |-- |={E}=> |> P.
-Proof.
-  intros; unfold cinvariant.
-(*  apply wsat_open.*)
-Admitted.
-
-Corollary cinv_cancel : forall E i g P, cinvariant i g P * cinv_own g Tsh |-- |={E}=> |> P.
+Lemma cinv_open : forall E sh i g P, readable_share sh -> Ensembles.In E i ->
+  cinvariant i g P * cinv_own g sh |-- |={E, Ensembles.Subtract E i}=> |> P * cinv_own g sh * (|> P -* |={Ensembles.Subtract E i, E}=> emp).
 Proof.
   intros.
-  apply wsat_fupd, cinv_cancel'.
+  unfold cinvariant.
+  sep_apply (inv_open E).
+  sep_apply fupd_frame_r; apply fupd_elim.
+  rewrite later_orp, !distrib_orp_sepcon; apply orp_left.
+  - eapply derives_trans, fupd_intro; cancel.
+    apply wand_derives; auto.
+    apply orp_right1; auto.
+  - eapply derives_trans, except_0_fupd.
+    apply orp_right1.
+    rewrite sepcon_assoc; eapply derives_trans; [apply sepcon_derives, now_later; apply derives_refl|].
+    rewrite <- later_sepcon; apply later_derives.
+    rewrite (sepcon_comm _ (cinv_own g sh)), <- sepcon_assoc.
+    rewrite sepcon_comm; apply sepcon_FF_derives'.
+    unfold cinv_own; sep_apply own_valid_2; Intros.
+    destruct H1 as (? & J & ?).
+    apply join_Tsh in J as []; subst; contradiction ghosts.unreadable_bot.
 Qed.
 
-Lemma cinv_open : forall i P,
-  wsat * cinvariant i P * ghost_set g_en (Ensembles.Singleton i) |--
-  (|==> wsat * |> P * ghost_list g_dis (list_singleton i (Some tt)))%I.
+Lemma cinvariant_nonexpansive : forall i g, nonexpansive (cinvariant i g).
 Proof.
-(* apply wsat_open. *)
-Admitted.
-
-(*Lemma wsat_close : forall i P,
-  wsat * invariant i P * |> P * ghost_list g_dis (list_singleton i (Some tt)) |--
-  (|==> wsat * ghost_set g_en (Ensembles.Singleton i))%I.
-Proof.
-  intros; unfold wsat, invariant.
-  iIntros "(((H & inv1) & HP) & dis1)". iDestruct "H" as (l lg lb) "((((% & inv) & dis) & en) & I)". iDestruct "inv1" as (g) "[snap agree]".
-  iAssert (!!(i < length lg /\ Znth (Z.of_nat i) lg = g /\
-    exists b, Znth (Z.of_nat i) lb = Some b)%nat) as %Hi.
-  { iCombine "snap inv" as "inv"; unfold master_list; erewrite snap_master_join1.
-    iDestruct "inv" as "[% inv]".
-    apply list_incl_singleton in H0.
-    destruct (lt_dec i (length lg));
-      [|erewrite nth_overflow in H0 by (erewrite map_length, upto_length; lia); discriminate].
-    erewrite nth_map' with (d' := 0) in H0 by (rewrite upto_length; lia).
-    erewrite nth_upto in H0 by lia.
-    destruct (Znth (Z.of_nat i) lb); inv H0; eauto. }
-  iDestruct "snap" as "_".
-  iModIntro.
-  destruct Hi as (? & ? & b & Hi).
-  assert (nth i lb None = Some b) as Hi' by (rewrite <- nth_Znth' in Hi; auto).
-  destruct b.
-  { iCombine "dis dis1" as "dis".
-    iDestruct (own_valid_2(RA := list_PCM _) with "[$dis]") as %H2.
-    destruct H2 as (? & J & _).
-    apply list_join_nth with (n := i) in J.
-    erewrite nth_singleton, nth_map' with (d' := None) in J by lia.
-    rewrite Hi' in J; inv J.
-    inv H5.
-    inv H3. }
-  erewrite ghost_set_remove with (a := i).
-  iDestruct "en" as "[$ en]".
-  iExists l, lg, (replace_nth i lb (Some true)).
-  rewrite replace_nth_length predicates_hered.prop_true_andp; last auto.
-  iSplitR "I agree HP".
-  iSplitR "en".
-  iSplitR "dis dis1".
-  - erewrite map_ext; [iFrame|].
-    intros.
-    destruct (eq_dec a (Z.of_nat i)); [subst; rewrite Znth_replace_nth | rewrite Znth_replace_nth'];
-      auto; try lia.
-    rewrite Hi; auto.
-  - iCombine "dis1 dis" as "dis"; setoid_rewrite <- own.ghost_op; [iFrame|].
-    rewrite map_replace_nth.
-    apply (list_join_singleton(P := token_PCM)).
-    { rewrite map_length; lia. }
-    erewrite nth_map' with (d' := None) by lia.
-    rewrite Hi'; constructor.
-  - erewrite Ensembles.Extensionality_Ensembles at 1; [iFrame|]; constructor; intros ? X.
-    + inv X; unfold Ensembles.In in *.
-      rewrite nth_replace_nth'; auto.
-      intro; subst; contradiction.
-    + constructor.
-      * unfold Ensembles.In in *.
-        destruct (eq_dec x i); [subst; auto|].
-        rewrite nth_replace_nth' in X; auto.
-      * intro X'; inv X'.
-        unfold Ensembles.In in X.
-        rewrite -> nth_replace_nth in X by lia; inv X.
-  - erewrite !iter_sepcon_eq, @iter_sepcon_Znth with (i := Z.of_nat i)
-      by (rewrite Zlength_upto; split; [|apply Nat2Z.inj_lt]; lia).
-    erewrite @iter_sepcon_Znth with (i := Z.of_nat i)(l := upto _)
-      by (rewrite Zlength_upto; split; [|apply Nat2Z.inj_lt]; lia).
-    erewrite !Znth_upto, !Znth_replace_nth by lia.
-    rewrite Hi.
-    iDestruct "I" as "[agree' I]".
-    subst; iDestruct (agree_join2 with "[agree' agree]") as "[imp agree]"; first by iFrame.
-    iPoseProof ("imp" with "HP") as "?"; iFrame.
-    erewrite iter_sepcon_func_strong; eauto.
-    unfold remove_Znth; intros ? Hin.
-    rewrite Znth_replace_nth'; auto.
-    intro; subst.
-    apply in_app in Hin as [?%In_sublist_upto | ?%In_sublist_upto]; lia.
-  - unfold Ensembles.In; auto.
-Qed.*)
-
-(*Lemma cinvariant_nonexpansive : forall N, nonexpansive (cinvariant N).
-Proof.
-  intros; unfold inv.
-  apply @exists_nonexpansive; intros i.
-  apply @conj_nonexpansive, invariant_nonexpansive.
-  apply const_nonexpansive.
+  intros; apply invariant_nonexpansive2.
+  apply @disj_nonexpansive, const_nonexpansive.
+  apply identity_nonexpansive.
 Qed.
 
-Lemma inv_nonexpansive2 : forall N f, nonexpansive f ->
-  nonexpansive (fun a => inv N (f a)).
+Lemma cinvariant_nonexpansive2 : forall i g f, nonexpansive f ->
+  nonexpansive (fun a => cinvariant i g (f a)).
 Proof.
-  intros; unfold inv.
-  apply @exists_nonexpansive; intros i.
-  apply @conj_nonexpansive, invariant_nonexpansive2, H.
-  apply const_nonexpansive.
-Qed.*)
+  intros; apply invariant_nonexpansive2.
+  apply @disj_nonexpansive, const_nonexpansive; auto.
+Qed.
 
 Lemma cinvariant_super_non_expansive : forall i g R n, compcert_rmaps.RML.R.approx n (cinvariant i g R) =
   compcert_rmaps.RML.R.approx n (cinvariant i g (compcert_rmaps.RML.R.approx n R)).
